pcuic/theories/PCUICSubstitution.v
@@ -350,6 +350,23 @@ Proof.
     + eapply typed_subst in t1 as [Ht HT]; eauto. lia.
 Qed.
 
+Lemma subst_declared_symbol `{checker_flags} :
+  forall Σ k n u decl ty i s,
+    wf Σ ->
+    declared_symbol Σ k decl ->
+    nth_error (symbols decl) n = Some ty ->
+    let ty' :=
+      subst_instance_constr u ((subst0 (symbols_subst k n u #|symbols decl|)) ty)
+    in
+    subst s i ty' = ty'.
+Proof.
+  intros Σ k n u decl ty i s hΣ h e ty'.
+  eapply subst_closedn.
+  eapply closed_upwards.
+  - eapply closed_declared_symbol. all: eauto.
+  - lia.
+Qed.
+
 Lemma subst_declared_constant `{H:checker_flags} Σ cst decl n k u :
   wf Σ ->
   declared_constant Σ cst decl ->
@@ -2059,6 +2076,9 @@ Proof.
   - specialize (X1 Γ Γ' Δ s sub eq_refl wfsubs).
     eapply refine_type. econstructor; eauto.
     unfold subst1. rewrite -> distr_subst. simpl. reflexivity.
+
+  - erewrite subst_declared_symbol by eassumption.
+    constructor. all: eauto.
 
   - eapply refine_type. constructor; eauto.
     rewrite !map_cst_type. eapply subst_declared_constant in H as ->; eauto.
