pcuic/theories/PCUICValidity.v
@@ -225,6 +225,8 @@ Section Validity.
         simpl in b. eapply cumul_trans. auto. 2:eauto.
         constructor. constructor. simpl. apply leq_universe_product. auto.
 
+    - admit.
+
     - (* eapply declared_constant_inv in H; pcuic.
       destruct decl as [ty [b|] univs]. red in H. simpl in *.
       destruct Σ as [Σ φ].
